test/identity_coercion.v
@@ -1,0 +1,13 @@
+Section uo.
+  Definition fct := nat -> nat.
+  Parameter incr_fct : Set.
+  Parameter fct_of_incr_fct : incr_fct -> fct.
+  
+  Fail Coercion fct_of_incr_fct : incr_fct >-> Funclass.
+  Coercion fct_of_incr_fct : incr_fct >-> fct.
+  Parameter f' : incr_fct.
+  Check f' : fct.
+  Fail Check f' 0.
+
+  Identity Coercion uo_fct_Funclass : fct >-> Funclass.
+  Check f' 0.
